concepts/Lax52.lean
@@ -1,9 +1,6 @@
 import Lax52.MSOSyntax
 import Lax52.MSOSemantics
 import Lax52.WordStructure
-import Lax52.MarkedWords
-import Lax52.ValidMarkedWordsRegular
-import Lax52.MSOFormulaRegularity
 import Lax52.NFARecognizable
 import Lax52.NFAToMSO
 import Lax52.MSOToNFA
